theories/simulations/gsim/GSimMod.v
@@ -1,0 +1,52 @@
+From CRIS.common Require Import Common ConcRA.
+From iris.proofmode Require Import proofmode.
+From CRIS.modules Require Import LMod Mod.
+From CRIS.simulations.gsim Require Import GSimAdequacy.
+
+Section GSIM_MOD.
+
+  Context `{!crisG Γ Σ α β τ _S _I}.
+
+  Program Definition gsim_mod_def (Ms Mt : Mod.t) : iProp Σ :=
+    {| uPred_holds := fun r =>
+                        Mod.wf Mt -> Mod.wf Ms /\
+                                      forall rt rs,
+                                        ✓ rs ->
+                                        (Own rs ⊢ Own rt ∗ Own r ∗ winv (∅,∅)) ->
+                                        gsim eq smj_bot smj_bot
+                                          (LMod.compile (Mod.to_lmod Ms rs) ()↑)
+                                          (LMod.compile (Mod.to_lmod Mt rt) ()↑)
+    |}.
+  Next Obligation.
+    intros Ms Mt x1 x2 H LE WFT. specialize (H WFT).
+    destruct H as [WFS H]. split; et.
+    intros rt rs VALID SPLIT. eapply H; et.
+    rewrite SPLIT.
+    iIntros "($ & H & $)". iApply Own_extends; et.
+  Qed.
+  Definition gsim_mod_aux : seal (@gsim_mod_def). Proof. by eexists. Qed.
+  Definition gsim_mod := gsim_mod_aux.(unseal).
+  Definition gsim_mod_unseal : @gsim_mod = @gsim_mod_def := gsim_mod_aux.(seal_eq).
+
+  Lemma gsim_mod_intro
+    Ms Mt P
+    (SIM : Mod.wf Mt -> Mod.wf Ms /\
+                         forall rt rs,
+                           ✓ rs ->
+                           (Own rs ⊢ Own rt ∗ P ∗ winv (∅,∅)) ->
+                           gsim eq smj_bot smj_bot
+                             (LMod.compile (Mod.to_lmod Ms rs) ()↑)
+                             (LMod.compile (Mod.to_lmod Mt rt) ()↑))
+    : P ⊢ gsim_mod Ms Mt.
+  Proof.
+    rewrite gsim_mod_unseal.
+    eapply entails_pointwise. intros r VALID HP.
+    eapply Own_general_completeness. cbn.
+    intros WFT. specialize (SIM WFT). destruct SIM as [WFS SIM].
+    split; et.
+    intros rt rs VRS SPLIT. eapply SIM; et.
+    rewrite SPLIT.
+    iIntros "($ & R & $)". iApply HP. done.
+  Qed.
+
+End GSIM_MOD.
