theories/simulations/lsim/LSimMod.v
@@ -1,0 +1,52 @@
+From CRIS.common Require Import Common ConcRA.
+From iris.proofmode Require Import proofmode.
+From CRIS.modules Require Import Mod.
+From CRIS.simulations.lsim Require Import LSim.
+
+Section LSIM_MOD.
+
+  Context `{!crisG Γ Σ α β τ _S _I}.
+
+  Program Definition lsim_mod_def (Ms Mt : Mod.t) : iProp Σ :=
+    {| uPred_holds := fun r =>
+        Mod.wf Mt ->
+        Mod.wf Ms /\
+          forall rt rs,
+            ✓ rs ->
+            (Own rs ⊢ Own rt ∗ Own r ∗ winv (∅,∅)) ->
+            ∃ lw, LSim.lsim_lmod
+              (Mod.to_lmod Ms rs) (Mod.to_lmod Mt rt) lw
+    |}.
+  Next Obligation.
+    intros Ms Mt x1 x2 H LE WFT. specialize (H WFT).
+    destruct H as [WFS H]. split; et.
+    intros rt rs VALID SPLIT. eapply H; et.
+    rewrite SPLIT.
+    iIntros "($ & H & $)". iApply Own_extends; et.
+  Qed.
+  Definition lsim_mod_aux : seal (@lsim_mod_def). Proof. by eexists. Qed.
+  Definition lsim_mod := lsim_mod_aux.(unseal).
+  Definition lsim_mod_unseal : @lsim_mod = @lsim_mod_def := lsim_mod_aux.(seal_eq).
+
+  Lemma lsim_mod_intro
+    Ms Mt P
+    (SIM : Mod.wf Mt ->
+      Mod.wf Ms /\
+        forall rt rs,
+          ✓ rs ->
+          (Own rs ⊢ Own rt ∗ P ∗ winv (∅,∅)) ->
+          ∃ lw, LSim.lsim_lmod
+            (Mod.to_lmod Ms rs) (Mod.to_lmod Mt rt) lw)
+    : P ⊢ lsim_mod Ms Mt.
+  Proof.
+    rewrite lsim_mod_unseal.
+    eapply entails_pointwise. intros r VALID HP.
+    eapply Own_general_completeness. cbn.
+    intros WFT. specialize (SIM WFT). destruct SIM as [WFS SIM].
+    split; et.
+    intros rt rs VRS SPLIT. eapply SIM; et.
+    rewrite SPLIT.
+    iIntros "($ & R & $)". iApply HP. done.
+  Qed.
+
+End LSIM_MOD.
