theories/simulations/msim/ISimAdequacy.v
@@ -1,6 +1,6 @@
 From CRIS.common Require Import Common ConcRA.
 From CRIS.modules Require Import LMod Mod SMod Sp.
-From CRIS.simulations.lsim Require Import LSim.
+From CRIS.simulations.lsim Require Import LSim LSimMod.
 From CRIS.simulations.msim Require Import MSimCommon MSim MSimAdequacy ISim ISimFacts TacticsCommon ITactics SimNotations.
 From iris.proofmode Require Import proofmode.
 From stdpp Require Import base list.
@@ -8,52 +8,100 @@ From stdpp Require Import base list.
 Section ISIM_ADEQUACY.
   Context `{_crisG: !crisG Γ Σ α β τ _S _I}.
 
-  Lemma ISim_wf contextual ms mt cond Ist :
-    ISim.t contextual ms mt cond Ist → Mod.wf mt → Mod.wf ms.
+  Lemma ISim_wf contextual ms mt Ist :
+    ISim.t contextual ms mt Ist ⊢
+      (⌜Mod.wf mt⌝ → ⌜Mod.wf ms⌝).
   Proof.
-    intros [] WFT. econs; et.
-    specialize (sim_scopes WFT).
+    rewrite /ISim.t.
+    iIntros "SIM %WFT".
+    iSpecialize ("SIM" with "[]"); first done.
+    iDestruct "SIM" as "[[%SCOPES %NODUP] _]".
+    iPureIntro. econs; et.
     eapply submseteq_NoDup; et. apply WFT.
   Qed.
   
-  Lemma ISim_dom contextual ms mt cond Ist :
-    ISim.t contextual ms mt cond Ist →
-    Mod.wf mt →
-    dom (Mod.fnsems ms) ⊆ dom (Mod.fnsems mt).
+  Lemma ISim_dom contextual ms mt Ist :
+    ISim.t contextual ms mt Ist ⊢
+      (⌜Mod.wf mt⌝ →
+       ⌜dom (Mod.fnsems ms) ⊆ dom (Mod.fnsems mt)⌝).
   Proof using.
-    intros Hsim Hwf fn [? Hin]%elem_of_dom; eapply ISim_wf in Hwf as Hwfsrc; eauto.
-    rewrite elem_of_dom.
-    destruct (_ mt !! fn) eqn : Ht; ss. exfalso.
-    destruct Hsim; hexploit (sim_fnsems Hwf fn); eauto.
-    rewrite /ISim.sim_fun ?lookup_fmap /= Hin /=. destruct x; s; i.
-    - hexploit H; et. i; des. rewrite Ht in H0. ss.
-    - eapply Hwfsrc in Hin. rr in Hin. des; ss.
+    eapply entails_pointwise. intros r VALID SIM.
+    assert (WFSIM :
+      Own r ⊢ ⌜Mod.wf mt⌝ → ⌜Mod.wf ms⌝).
+    { rewrite SIM. eapply ISim_wf. }
+    iIntros "R %WFT". iStopProof.
+    assert (WFS : Mod.wf ms).
+    { eapply Own_pure_soundness; et. rewrite WFSIM.
+      iIntros "SIM". iApply "SIM". done. }
+    assert (DOM : dom (Mod.fnsems ms) ⊆ dom (Mod.fnsems mt)).
+    { intros fn [f Hin]%elem_of_dom.
+      rewrite elem_of_dom.
+      destruct f as [[msk body]|].
+      - assert (TGT :
+          ∃ ft,
+            sandbox_fnsemmap (Mod.fnsems mt) !! fn =
+              Some (Some ft)).
+        { eapply Own_pure_soundness; et. rewrite SIM /ISim.t.
+          iIntros "SIM".
+          iSpecialize ("SIM" with "[]"); first done.
+          iDestruct "SIM" as "[_ [_ FUNS]]".
+          rewrite /ISim.sim_fun.
+          iSpecialize ("FUNS" $! fn with "[] []").
+          { done. }
+          { done. }
+          iSpecialize ("FUNS" $! (SB.sandbox_body (msk, body))
+            with "[]").
+          { iPureIntro.
+            rewrite /sandbox_fnsemmap lookup_fmap Hin //. }
+          iDestruct "FUNS" as (ft) "[%Hft _]".
+          iPureIntro. eauto. }
+        destruct TGT as [ft Hft].
+        rewrite /sandbox_fnsemmap lookup_fmap in Hft.
+        destruct (Mod.fnsems mt !! fn); ss; eauto.
+      - exfalso. eapply WFS in Hin. rr in Hin. des; ss. }
+    iIntros "_". iPureIntro. exact DOM.
   Qed.
 
-  (* ISim.t implies lsim_lmod *)
-  Lemma ISim_adequacy (ms mt : Mod.t) (rs rt : Σ) (IC : iProp Σ) Ist
-      (SUB : Own rs ⊢ |==> Own rt ∗ (IC ∗ winv (∅,∅)))
-      (WF : ✓ rs)
-      (WFT : Mod.wf mt)
-      (SIM : ISim.t closed ms mt IC Ist) :
-    lsim_lmod
-      (Mod.to_lmod ms rs) (Mod.to_lmod mt rt)
-      (IstWorld (λ x y, winv (∅, ∅) ∗ Ist x y)%I).
+  (* ISim.t implies lsim_mod *)
+  Lemma ISim_adequacy
+    (ms mt : Mod.t) Ist
+    : ISim.t closed ms mt Ist ⊢ lsim_mod ms mt.
   Proof using.
-    hexploit ISim_wf; eauto; intros WFS.
-    dup SIM. dup WFS. dup WFT. destruct SIM0, WFS0, WFT0.
-    eapply Own_bupd_split in SUB as
-      [rrt [rinit [SUB [HRT HINIT]]]]; eauto.
+    eapply entails_pointwise. intros r VALID SIM.
+    rewrite lsim_mod_unseal.
+    eapply Own_general_completeness. cbn.
+    intros WFT.
+    assert (WFS : Mod.wf ms).
+    { eapply Own_pure_soundness; et.
+      rewrite SIM. iIntros "SIM".
+      iPoseProof (ISim_wf with "SIM") as "WF".
+      iApply "WF". done. }
+    split; first done.
+    intros rt rs WF SUB.
+    exists (IstWorld (λ x y,
+      (∀ fn, ISim.sim_fun closed ms mt Ist fn) ∗
+        winv (∅, ∅) ∗ Ist x y)%I).
+    dup WFS. dup WFT. destruct WFS0, WFT0.
+    assert (SUB' : Own rs ⊢ |==> Own rt ∗
+      ((∀ fn, ISim.sim_fun closed ms mt Ist fn) ∗
+        winv (∅, ∅) ∗
+        Ist (Mod.initial_st ms) (Mod.initial_st mt))).
+    { rewrite SUB SIM /ISim.t.
+      iIntros "($ & SIM & WINV)".
+      iSpecialize ("SIM" with "[]"); first done.
+      iDestruct "SIM" as "[_ [INIT FUNS]]".
+      iModIntro. iFrame. }
+    eapply Own_bupd_split in SUB' as
+      [rrt [rinit [SUBOWN [HRT HINIT]]]]; eauto.
     constructor; ss.
     - eapply interp_inv_intro with (mr := rinit).
       + exact WF.
-      + iIntros "H". iMod (SUB with "H") as "[RT INIT]".
+      + iIntros "H". iMod (SUBOWN with "H") as "[RT INIT]".
         rewrite /ctx_sem /= left_id Own_op.
         iModIntro. iSplitL "INIT"; first done.
         iApply HRT; done.
       + iIntros "INIT". iModIntro.
-        iPoseProof (HINIT with "INIT") as "[IC WINV]".
-        iFrame "WINV". iApply sim_initial; done.
+        iApply HINIT; done.
       + destruct ms; ss; apply nodup_init; eauto.
       + destruct mt; ss; apply nodup_init; eauto.
     - ii; inv WF0. econs; eauto.
@@ -61,26 +109,62 @@ Section ISIM_ADEQUACY.
       unfold ctx_sem. rewrite big_opL_app. s. rewrite ?right_id; eauto.
     - intros fn fs; rewrite ?lookup_fmap lookup_omap.
       destruct (_ ms !! fn) as [[[msks its]|]|] eqn : Hms; ss; i; clarify.
-      hexploit (sim_fnsems WFT fn); eauto.
-      rewrite /ISim.sim_fun ?lookup_fmap Hms /= ?lookup_fmap lookup_omap.
-      intros H; hexploit H; clear H; eauto.
-      destruct (_ mt !! fn) as [[[mskt itt]|]|] eqn : Hmt;
-        try by (i; des; clarify).
-      intros [? [? Hsim]]; clarify; ss.
-      eexists; split; first done.
-      intros tid ??? arg ??. inv SIMMRS. specialize (Hsim arg st_src st_tgt).
+      assert (TGT :
+        ∃ ft,
+          sandbox_fnsemmap (Mod.fnsems mt) !! fn =
+            Some (Some ft)).
+      { eapply Own_pure_soundness with (a := r); et.
+        rewrite SIM /ISim.t.
+        iIntros "SIM".
+        iSpecialize ("SIM" with "[]"); first done.
+        iDestruct "SIM" as "[_ [_ FUNS]]".
+        rewrite /ISim.sim_fun.
+        iSpecialize ("FUNS" $! fn with "[] []").
+        { done. }
+        { done. }
+        iSpecialize ("FUNS" $! (SB.sandbox_body (msks, its))
+          with "[]").
+        { iPureIntro.
+          rewrite /sandbox_fnsemmap lookup_fmap Hms //. }
+        iDestruct "FUNS" as (ft) "[%Hft _]".
+        iPureIntro. eauto. }
+      destruct TGT as [ft Hft].
+      rewrite /sandbox_fnsemmap lookup_fmap in Hft.
+      destruct (_ mt !! fn) as [[[mskt itt]|]|] eqn : Hmt; ss;
+        clarify.
+      eexists (ModTr.trans_fnsem (SB.sandbox_body (mskt, itt))).
+      split.
+      { rewrite ?lookup_fmap lookup_omap Hmt //. }
+      intros tid ??? arg ??. inv SIMMRS.
       eapply msim_adequacy; eauto; cycle 4.
       { apply le_mine_refl. }
       { ginit; cycle 2; i.
         eapply gpaco8_mon with (r := bot8) (rg:= iunlift ibot); eauto using iunlift_ibot.
         eapply isim_init; eauto.
-        iIntros "H". iApply isim_upd. iMod (MR with "H") as "[I H]".
-        iPoseProof (Hsim with "[H]") as "SIM"; cycle 2; s; et.
+        iIntros "H". iApply isim_upd.
+        iMod (MR with "H") as "[FUNS [I H]]".
+        iDestruct "FUNS" as "#FUNS".
+        iPoseProof "FUNS" as "FSIM".
+        iEval (rewrite /ISim.sim_fun) in "FSIM".
+        iSpecialize ("FSIM" $! fn with "[] []").
+        { done. }
+        { done. }
+        iSpecialize ("FSIM" $! (SB.sandbox_body (msks, its))
+          with "[]").
+        { iPureIntro.
+          rewrite /sandbox_fnsemmap lookup_fmap Hms //. }
+        iDestruct "FSIM" as (ft') "[%Hft' Hsim]".
+        rewrite /sandbox_fnsemmap lookup_fmap Hmt /= in Hft'.
+        clarify.
+        rewrite /isim_fsem.
+        iSpecialize ("Hsim" $! arg st_src st_tgt with "H").
         iPoseProof (winv_split_empty with "[I]") as "[I I']"; et.
-        iPoseProof ("SIM" with "I") as "SIM".
+        iPoseProof ("Hsim" with "I") as "ISIM".
         iModIntro. iApply isim_mono; cycle 1; i.
-        { iApply isim_ist_frame; et. iFrame. }
-        { s. iIntros "[? [? ?]]". iFrame. }
+        { iApply isim_ist_frame.
+          iSplitL "FUNS". { iFrame "FUNS". }
+          iApply isim_ist_frame. iFrame "I' ISIM". }
+        { s. iIntros "[FUNS [WINV [EQ IST]]]". iFrame. }
       }
       { f_equal. apply map_eq; intros i; rewrite ?lookup_omap ?lookup_fmap lookup_omap.
         destruct (_ ms !! i); ss.
