theories/simulations/msim/TacticsInit.v
@@ -1,9 +1,31 @@
 From CRIS.common Require Import Common ConcRA.
 From iris.proofmode Require Export proofmode.
-From CRIS.simulations.msim Require Import TacticsCommon ITactics WTactics Tactics ISim ISimFacts WSim.
+From CRIS.simulations.msim Require Export FnsemLookup.
+From CRIS.simulations.msim Require Import
+  TacticsCommon ITactics WTactics Tactics ISim ISimFacts WSim.
 From CRIS.modules Require Import Mod SModTr.
 
+Ltac rewrite_fnsem_lookup_in fl fn H :=
+  let Hlookup := fresh "Hlookup" in
+  first
+    [ assert (Hlookup : FnsemLookupResult fl fn _) by
+        solve [once (typeclasses eauto with fnsem_lookup)];
+      destruct Hlookup as [Hlookup];
+      rewrite Hlookup in H; clear Hlookup
+    | let fl' := fnsem_lookup_normalize_map fl in
+      let Hrhs :=
+        lazymatch type of H with
+        | _ = ?Hrhs => Hrhs
+        end in
+      change (fl' !! fn = Hrhs) in H;
+      assert (Hlookup : FnsemLookupResult fl' fn _) by
+        solve [once (typeclasses eauto with fnsem_lookup)];
+      destruct Hlookup as [Hlookup];
+      rewrite Hlookup in H; clear Hlookup
+    ].
+
 Ltac cStartModSim :=
+  first [ unfold bi_emp_valid | idtac ];
   (first
     [ eapply ISim_reflR;
       [ intros fn Hfn; (repeat rewrite Mod.dom_fnsems_add in Hfn); set_unfold in Hfn; des; subst
@@ -12,27 +34,70 @@ Ltac cStartModSim :=
       | ((set_unfold; naive_solver) || (try timeout 1 mod_tac))
       | try timeout 1 mod_tac
       |]
-    | econs; intros Hwf;
-      [ (refl||eauto using submseteq_nil_l)
-      | try timeout 1 mod_tac
-      |
-      | intros fn; eapply ISim.sim_fun_strong; intros Hfn; (repeat rewrite Mod.dom_fnsems_add in Hfn); set_unfold in Hfn; des; subst
-      ]
+    | lazymatch goal with
+      | |- ?P ⊢ ISim.t ?ctx ?ms_src ?ms_tgt ?Ist =>
+          rewrite /ISim.t;
+          iIntros "INIT" (Hwf);
+          iSplit;
+          [ iPureIntro; split;
+            [ (refl||eauto using submseteq_nil_l)
+            | try timeout 1 mod_tac
+            ]
+          | iSplitL "INIT";
+            [ iRevert "INIT"
+            | let fn := fresh "fn" in
+              iIntros (fn);
+              destruct (decide (fn ∈ dom (Mod.fnsems ms_src)))
+                as [Hfn|Hfn];
+              [ (repeat rewrite Mod.dom_fnsems_add in Hfn);
+                set_unfold in Hfn; des; subst
+              | rewrite /ISim.sim_fun;
+                iIntros "%WFS %WFT2" (fs) "%";
+                match goal with
+                | Hfs : _ !! fn = Some (Some _) |- _ =>
+                    iExFalso; iPureIntro; apply Hfn;
+                    apply elem_of_dom_2 in Hfs;
+                    rewrite /sandbox_fnsemmap dom_fmap in Hfs; done
+                end
+              ]
+            ]
+          ]
+      end
     ]).
 
 Ltac cStartFunSim :=
+  iStartProof;
   lazymatch goal with
-  | |- ISim.sim_fun ?ctx ?ms_src ?ms_tgt ?Ist ?fn =>
-      let wfs := fresh "WFS" in
-      let wft := fresh "WFT" in
-      rewrite /ISim.sim_fun; intros wfs wft;
+  | |- environments.envs_entails _
+        (ISim.sim_fun _ _ _ _ _) => idtac
+  | |- environments.envs_entails _
+        (_ -∗ ISim.sim_fun _ _ _ _ _) =>
+      first [ iIntros "#?" | iIntros "?" ]
+  end;
+  lazymatch goal with
+  | |- environments.envs_entails _
+        (ISim.sim_fun ?ctx ?ms_src ?ms_tgt ?Ist ?fn) =>
+      rewrite /ISim.sim_fun;
+      iIntros "%WFS %WFT" (fs);
       first
-        [ rewrite_fnsem_lookup
-            (sandbox_fnsemmap (Mod.fnsems ms_src)) fn;
-          eexists
-        | simpl_map; eexists
+        [ iIntros "%";
+          match goal with
+          | Hfs : _ = Some (Some _) |- _ =>
+              rewrite_fnsem_lookup_in
+                (sandbox_fnsemmap (Mod.fnsems ms_src)) fn Hfs;
+              simplify_eq
+          end
+        | simpl_map;
+          iIntros "%";
+          match goal with
+          | Hfs : _ = Some (Some _) |- _ =>
+              cbn in Hfs; simplify_eq
+          end
         ];
-      split; first prove_inline_cond;
+      iExists _;
+      iSplit; first (iPureIntro; prove_inline_cond);
+      rewrite /isim_fsem;
+      iModIntro;
       iIntros (arg st_src st_tgt) "IST"; iApply wsim_isim;
       rewrite /SB.sandbox_body; simpl fst; simpl snd;
       rewrite /SModTr.trans_fnsem /SModTr.HoareFun /cfunU /cfunN
